Auto/Embedding/LamConv.lean
@@ -2,191 +2,6 @@ import Auto.Embedding.LamBase
 
 namespace Auto.Embedding.Lam
 
-private def LamTerm.bvarLiftsIdxRec (idx : Nat) (t : LamTerm) : (lvl : Nat) → LamTerm
-| 0 => t
-| lvl' + 1 => (t.bvarLiftsIdxRec idx lvl').bvarLiftIdx idx
-
-private def LamTerm.bvarLiftsRec := LamTerm.bvarLiftsIdxRec 0
-
-private def LamWF.ofBVarLiftIdxRec_bvarAux
-  (lctx : Nat → α) (pos n : Nat) :
-  pushLCtxAtRec lctx x pos (popLCtxAtRec id pos n) = lctx n := by
-  rw [popLCtxAtRec.comm id (pushLCtxAtRec lctx x pos)]; dsimp
-  rw [popAtRec_pushAtRec_eq]
-
-private def LamWF.ofBVarLiftIdxRec {lamVarTy lctx} (idx : Nat) (rterm : LamTerm) :
-  (HWF : LamWF lamVarTy ⟨lctx, rterm, rTy⟩) →
-  LamWF lamVarTy ⟨pushLCtxAtRec lctx x idx, rterm.bvarLiftIdx idx, rTy⟩
-| .ofAtom n => .ofAtom n
-| .ofBase b => .ofBase b
-| .ofBVar n => 
-  let IH := @LamWF.ofBVar lamVarTy (pushLCtxAtRec lctx x idx) (popLCtxAtRec id idx n)
-  LamWF.ofBVarLiftIdxRec_bvarAux lctx idx _ ▸ IH
-| .ofLam (argTy:=argTy) (body:=body) bodyTy wfBody =>
-  .ofLam (argTy:=argTy) bodyTy
-    (body:=body.bvarLiftIdx (Nat.succ idx))
-    (LamWF.ofBVarLiftIdxRec (lctx:=pushLCtx lctx argTy) (Nat.succ idx) _ wfBody)
-| .ofApp argTy' HFn HArg =>
-  let IHFn := LamWF.ofBVarLiftIdxRec idx _ HFn
-  let IHArg := LamWF.ofBVarLiftIdxRec idx _ HArg
-  .ofApp argTy' IHFn IHArg
-
-private def LamWF.ofBVarLiftRec {lamVarTy lctx} (rterm : LamTerm) 
-  (HWF : LamWF lamVarTy ⟨lctx, rterm, rTy⟩) :
-  LamWF lamVarTy ⟨pushLCtx lctx x, rterm.bvarLiftRec, rTy⟩ :=
-  LamWF.ofBVarLiftIdxRec 0 rterm HWF
-
-private def LamWF.bvarLiftIdxRec.correct_bvarAux {rty : Nat → α}
-  {lctxty : α → Sort u} (lctx : ∀ n, lctxty (rty n))
-  {xty : α} (x : lctxty xty) (pos n : Nat) :
-  HEq (pushLCtxAtDepRec lctx x pos (popLCtxAtRec id pos n)) (lctx n) := by
-  rw [popLCtxAtRec.commDep id (pushLCtxAtDepRec lctx x pos)]; simp
-  apply HEq.trans
-    (b := @popLCtxAtDepRec _ (pushLCtxAtRec rty xty pos) lctxty (fun n => pushLCtxAtDepRec lctx x pos n) pos n)
-  case h₁ => apply HEq.symm; apply @popLCtxAtDepRec.absorbAux'
-  case h₂ => apply popAtDepRec_pushAtDepRec_eq
-
-private def LamWF.bvarLiftIdxRec.correct.{u}
-  (lval : LamValuation.{u}) (lctxTy : Nat → LamSort) (idx : Nat)
-  (lctxTerm : ∀ n, (lctxTy n).interp lval.ilVal.tyVal)
-  {xty : LamSort} (x : LamSort.interp lval.ilVal.tyVal xty) :
-  (rterm : LamTerm) → (HWF : LamWF lval.ilVal.toLamTyVal ⟨lctxTy, rterm, rTy⟩) →
-  LamWF.interp lval lctxTy lctxTerm HWF = LamWF.interp lval
-    (pushLCtxAtRec lctxTy xty idx) (pushLCtxAtDepRec lctxTerm x idx)
-    (ofBVarLiftIdxRec idx rterm HWF)
-| .atom n, .ofAtom _ => rfl
-| .base _, .ofBase _ => rfl
-| .bvar n, .ofBVar _ => by
-  dsimp [LamWF.interp, ofBVarLiftIdxRec];
-  apply eq_of_heq
-  apply HEq.trans (b:=LamWF.interp lval
-    (pushLCtxAtRec lctxTy xty idx) (pushLCtxAtDepRec lctxTerm x idx)
-    (ofBVar (popLCtxAtRec id idx n)))
-  case h.h₁ =>
-    dsimp [LamWF.interp]
-    apply HEq.symm; apply LamWF.bvarLiftIdxRec.correct_bvarAux
-  case h.h₂ =>
-    apply LamWF.interp.heq <;> try rfl
-| .lam argTy body, .ofLam bodyTy wfBody => funext (fun x' => LamWF.bvarLiftIdxRec.correct
-    lval (pushLCtx lctxTy argTy) (Nat.succ idx)
-    (pushLCtxDep lctxTerm x') x body wfBody)
-| .app fn arg, .ofApp argTy HFn HArg => by
-  dsimp [LamWF.interp]
-  let IHFn := LamWF.bvarLiftIdxRec.correct lval lctxTy idx lctxTerm x fn HFn
-  let IHArg := LamWF.bvarLiftIdxRec.correct lval lctxTy idx lctxTerm x arg HArg
-  rw [IHFn]; rw [IHArg]
-
-def LamWF.bvarLiftRec.correct.{u}
-  (lval : LamValuation.{u}) (lctxTy : Nat → LamSort)
-  (lctxTerm : ∀ n, (lctxTy n).interp lval.ilVal.tyVal)
-  {xty : LamSort} (x : LamSort.interp lval.ilVal.tyVal xty) :
-  (rterm : LamTerm) → (HWF : LamWF lval.ilVal.toLamTyVal ⟨lctxTy, rterm, rTy⟩) →
-  LamWF.interp lval lctxTy lctxTerm HWF = LamWF.interp lval
-    (pushLCtx lctxTy xty) (pushLCtxDep lctxTerm x)
-    (ofBVarLiftRec rterm HWF) :=
-  LamWF.bvarLiftIdxRec.correct lval lctxTy 0 lctxTerm x
-
--- Suppose we have `(λ x. func[body]) arg`
---   and `body` is a subterm of `func` under `idx` levels of binders in `func`.
---   We want to compute what `body` will become when we beta-reduce the whole term
--- `bj` is the judgement related to the body, i.e. `lctx ⊢ body : ty`. It's
---   easy to see that the `lctx` which `arg` resides in is `fun n => lctx (n + idx + 1)`
---   and the type of `arg` is `lctx idx`
-private def LamWF.subst' (ltv : LamTyVal) (idx : Nat)
-  {arg : LamTerm} {argTy : LamSort}
-  {body : LamTerm} {bodyTy : LamSort} :
-  (lctx : Nat → LamSort) → 
-  (wfArg : LamWF ltv ⟨lctx, LamTerm.bvarLiftsRec arg idx, argTy⟩) →
-  (wfBody : LamWF ltv ⟨pushLCtxAtRec lctx argTy idx, body, bodyTy⟩) →
-  (substed : LamTerm) × LamWF ltv ⟨lctx, substed, bodyTy⟩
-| lctx, _,     .ofAtom n => ⟨.atom n, .ofAtom _⟩
-| lctx, _,     .ofBase (b:=b) H => ⟨.base b, .ofBase H⟩
-| lctx, wfArg, .ofBVar n =>
-  let lctxty := fun rty => (substed : LamTerm) × LamWF ltv { lctx := lctx, rterm := substed, rty := rty}
-  let arg' := LamTerm.bvarLiftsRec arg idx
-  pushLCtxAtDepRec (rty:=lctx) (lctxty:=lctxty) (lctx := fun n => ⟨.bvar n, .ofBVar n⟩) (xty:=argTy) (x := ⟨arg', wfArg⟩) idx n
-| lctx, wfArg, .ofLam (argTy:=argTy') bodyTy' (body:=body') H =>
-  let wfArg' := LamWF.ofBVarLiftRec (lctx:=lctx) _ wfArg
-  let IHArg := LamWF.subst' ltv (Nat.succ idx) _ wfArg' H
-  ⟨.lam argTy' IHArg.fst, .ofLam _ IHArg.snd⟩
-| lctx, wfArg, .ofApp argTy' HFn HArg =>
-  let IHFn := LamWF.subst' ltv idx _ wfArg HFn
-  let IHArg := LamWF.subst' ltv idx _ wfArg HArg
-  ⟨.app IHFn.fst IHArg.fst, .ofApp argTy' IHFn.snd IHArg.snd⟩
-
-private def LamWF.subst'.correct.{u}
-  (lval : LamValuation.{u}) (idx : Nat)
-  {arg : LamTerm} {argTy : LamSort} {body : LamTerm} {bodyTy : LamSort} :
-  (lctxTy : Nat → LamSort) → (lctxTerm : ∀ n, (lctxTy n).interp lval.ilVal.tyVal) →
-  (wfArg : LamWF lval.ilVal.toLamTyVal ⟨lctxTy, LamTerm.bvarLiftsRec arg idx, argTy⟩) →
-  (wfBody : LamWF lval.ilVal.toLamTyVal ⟨pushLCtxAtRec lctxTy argTy idx, body, bodyTy⟩) →
-  let wfSubst' := LamWF.subst' lval.ilVal.toLamTyVal idx lctxTy wfArg wfBody
-  (LamWF.interp lval (pushLCtxAtRec lctxTy argTy idx)
-    (pushLCtxAtDepRec lctxTerm (LamWF.interp lval lctxTy lctxTerm wfArg) idx) wfBody
-  = LamWF.interp lval lctxTy lctxTerm wfSubst'.snd)
-| lctxTy, lctxTerm, wfArg, .ofAtom n => rfl
-| lctxTy, lctxTerm, wfArg, .ofBase b => rfl
-| lctxTy, lctxTerm, wfArg, .ofBVar n =>
-  let β := LamSort.interp lval.ilVal.tyVal
-  let lctxty := fun (rty : LamSort) => (t : LamTerm) × LamWF lval.ilVal.toLamTyVal ⟨lctxTy, t, rty⟩
-  let f := fun (rty : LamSort) (r : lctxty rty) => LamWF.interp lval lctxTy lctxTerm r.snd
-  let lctx := fun n => (⟨LamTerm.bvar n, .ofBVar n⟩ : @Sigma LamTerm
-    (fun substed => LamWF lval.ilVal.toLamTyVal ⟨lctxTy, substed, lctxTy n⟩))
-  Eq.symm (pushLCtxAtDepRec.comm (β:=β) (lctxty:=lctxty) f lctx ⟨_, wfArg⟩ _ _)
-| lctxTy, lctxTerm, wfArg, .ofLam (argTy:=argTy') bodyTy' (body:=body') H =>
-  funext (fun x =>
-    let wfArg' := LamWF.ofBVarLiftRec (lctx:=lctxTy) _ wfArg
-    let IH := LamWF.subst'.correct lval (.succ idx) (pushLCtx lctxTy argTy') (pushLCtxDep lctxTerm x) wfArg' H
-    Eq.trans (by
-      dsimp [LamWF.interp]
-      rw [← LamWF.bvarLiftRec.correct]
-      rfl) IH)
-| lctxTy, lctxTerm, wfArg, .ofApp argTy' HFn HArg =>
-  let IHFn := LamWF.subst'.correct lval idx lctxTy lctxTerm wfArg HFn
-  let IHArg := LamWF.subst'.correct lval idx lctxTy lctxTerm wfArg HArg
-  by dsimp [LamWF.interp]; dsimp at IHFn; dsimp at IHArg; simp [IHFn, IHArg]
-
-private def LamTerm.bvarLiftsIdx.equiv (idx : Nat) (t : LamTerm) (lvl : Nat) :
-  LamTerm.bvarLiftsIdxRec idx t lvl = LamTerm.bvarLiftsIdx idx t lvl := by
-  revert idx; revert t; induction lvl <;> intro t
-  case zero => dsimp [bvarLiftsIdxRec]; intro idx; rw [LamTerm.bvarLiftsIdx.zero]
-  case succ lvl' IHlvl =>
-    induction t <;> intro idx
-    case atom n =>
-      dsimp [bvarLiftsIdxRec, bvarLiftsIdx]
-      rw [IHlvl]; rfl
-    case base b =>
-      dsimp [bvarLiftsIdxRec, bvarLiftsIdx]
-      rw [IHlvl]; rfl
-    case bvar n =>
-      dsimp [bvarLiftsIdxRec, bvarLiftsIdx]; rw [IHlvl];
-      dsimp [bvarLiftsIdx, bvarLiftIdx]; apply congr_arg LamTerm.bvar
-      rw [popLCtxAt.equiv]; rw [popLCtxsAt.comm (popLCtxAt id idx)]; dsimp
-      apply Eq.symm; apply popLCtxsAt.succ_l
-    case lam s t IH =>
-      dsimp [bvarLiftsIdx, bvarLiftsIdxRec];
-      rw [IHlvl]; dsimp [bvarLiftsIdx, bvarLiftIdx, bvarLiftsIdx]; rw [← IHlvl];
-      dsimp [bvarLiftsIdxRec] at IH; rw [IH]
-    case app fn arg IHFn IHArg =>
-      simp [bvarLiftsIdxRec, bvarLiftsIdx];
-      rw [IHlvl]; dsimp [bvarLiftsIdx, bvarLiftIdx];
-      rw [← IHlvl fn]; rw [← IHlvl arg];
-      dsimp [bvarLiftsIdxRec] at IHFn; rw [IHFn]
-      dsimp [bvarLiftsIdxRec] at IHArg; rw [IHArg]
-
-def LamTerm.bvarLifts (t : LamTerm) (lvl : Nat) := LamTerm.bvarLiftsIdx 0 t lvl 
-
-def LamTerm.bvarLifts.zero (t : LamTerm) : LamTerm.bvarLifts t 0 = t :=
-  LamTerm.bvarLiftsIdx.zero 0 t
-
-def LamTerm.bvarLifts.succ (t : LamTerm) (lvl : Nat) :
-  LamTerm.bvarLifts t (.succ lvl) = LamTerm.bvarLiftRec (LamTerm.bvarLifts t lvl) :=
-  LamTerm.bvarLiftsIdx.succ _ _ _
-
-private def LamTerm.bvarLifts.equiv (t : LamTerm) (lvl : Nat) :
-  LamTerm.bvarLiftsRec t lvl = LamTerm.bvarLifts t lvl :=
-  LamTerm.bvarLiftsIdx.equiv 0 t lvl
-
 -- Suppose we have `(λ x. func[body]) arg`
 --   and `body` is a subterm of `func` under `idx` levels of binders in `func`.
 --   We want to compute what `body` will become when we beta-reduce the whole term
@@ -196,94 +11,96 @@ private def LamTerm.bvarLifts.equiv (t : LamTerm) (lvl : Nat) :
 def LamTerm.subst (idx : Nat) (arg : LamTerm) : (body : LamTerm) → LamTerm
 | .atom n      => .atom n
 | .base b      => .base b
-| .bvar n      => pushLCtxAt LamTerm.bvar (arg.bvarLifts idx) idx n
+| .bvar n      => pushLCtxAt (arg.bvarLifts idx) idx LamTerm.bvar n
 | .lam s body  => .lam s (LamTerm.subst (.succ idx) arg body)
 | .app fn arg' => .app (LamTerm.subst idx arg fn) (LamTerm.subst idx arg arg')
 
-private def LamTerm.subst.equiv (ltv : LamTyVal) (idx : Nat)
+private def LamWF.subst
+  (ltv : LamTyVal) (idx : Nat)
   {arg : LamTerm} {argTy : LamSort}
-  {body : LamTerm} {bodyTy : LamSort}
-  (lctx : Nat → LamSort) :
-  (wfArg : LamWF ltv ⟨lctx, LamTerm.bvarLiftsRec arg idx, argTy⟩) →
-  (wfBody : LamWF ltv ⟨pushLCtxAtRec lctx argTy idx, body, bodyTy⟩) →
-  LamTerm.subst idx arg body = (LamWF.subst' ltv idx lctx wfArg wfBody).fst
-| wfArg, .ofAtom n => rfl
-| _,     .ofBase (b:=b) H => rfl
-| wfArg, .ofBVar n => by
-  dsimp [LamTerm.subst, LamWF.subst']
-  let f := fun (x : LamSort) (t : (substed : LamTerm) × LamWF ltv ⟨lctx, substed, x⟩) => t.fst
-  let β₀ := fun ty substed => LamWF ltv ⟨lctx, substed, ty⟩
-  let lctx' := fun n => @Sigma.mk LamTerm (β₀ _) (LamTerm.bvar n) (@LamWF.ofBVar ltv lctx n)
-  let x := @Sigma.mk LamTerm (β₀ _) (bvarLiftsRec arg idx) wfArg
-  let GEq := @pushLCtxAtDepRec.comm _ _ lctx _ f lctx' _ x idx n
-  simp at GEq; rw [GEq]; rw [pushLCtxAtDepRec.nonDep]
-  rw [pushLCtxAt.equiv]; rw [LamTerm.bvarLifts.equiv]
-| wfArg, .ofLam (argTy:=argTy') bodyTy' (body:=body') H => by
-  dsimp [LamTerm.subst, LamWF.subst'];
-  rw [← @LamTerm.subst.equiv ltv (.succ idx) arg argTy body' bodyTy']
-| wfArg, .ofApp argTy' HFn HArg => by
-  dsimp [LamTerm.subst, LamWF.subst']
-  rw [← LamTerm.subst.equiv ltv idx lctx wfArg HFn]
-  rw [← LamTerm.subst.equiv ltv idx lctx wfArg HArg]
+  {body : LamTerm} {bodyTy : LamSort} :
+  (lctx : Nat → LamSort) → 
+  (wfArg : LamWF ltv ⟨lctx, arg.bvarLifts idx, argTy⟩) →
+  (wfBody : LamWF ltv ⟨pushLCtxAt argTy idx lctx, body, bodyTy⟩) →
+  LamWF ltv ⟨lctx, LamTerm.subst idx arg body, bodyTy⟩
+| lctx, _,     .ofAtom n => .ofAtom _
+| lctx, _,     .ofBase (b:=b) H => .ofBase H
+| lctx, wfArg, .ofBVar n => by
+  dsimp [LamTerm.subst, pushLCtxAt, restoreAt, pushLCtx]
+  match Nat.ble idx n with
+  | true =>
+    dsimp;
+    match (n - idx) with
+    | 0 => exact wfArg
+    | _ + 1 => exact .ofBVar _
+  | false => exact .ofBVar n
+| lctx, wfArg, .ofLam (argTy:=argTy') bodyTy' (body:=body') H =>
+  let wfArg' := LamWF.ofBVarLiftIdx (s:=argTy') (lctx:=lctx) 0 _ wfArg
+  let IHArg := LamWF.subst ltv (Nat.succ idx) _
+    (by
+      rw [pushLCtxAt.zero] at wfArg'
+      dsimp [LamTerm.bvarLifts] at wfArg'
+      rw [← LamTerm.bvarLiftsIdx.succ_r] at wfArg'
+      exact wfArg')
+    (by
+      rw [pushLCtx_pushLCtxAt] at H
+      exact H)
+  .ofLam _ IHArg
+| lctx, wfArg, .ofApp argTy' HFn HArg =>
+  let IHFn := LamWF.subst ltv idx _ wfArg HFn
+  let IHArg := LamWF.subst ltv idx _ wfArg HArg
+  .ofApp argTy' IHFn IHArg
 
-def LamWF.ofBVarLift {lamVarTy lctx} (rterm : LamTerm) 
-  (HWF : LamWF lamVarTy ⟨lctx, rterm, rTy⟩) :
-  LamWF lamVarTy ⟨pushLCtx lctx x, rterm.bvarLifts 1, rTy⟩ := by
-  rw [← LamTerm.bvarLifts.equiv]; apply LamWF.ofBVarLiftRec _ HWF
-
-def LamWF.subst (ltv : LamTyVal) (idx : Nat)
-  {arg : LamTerm} {argTy : LamSort}
-  {body : LamTerm} {bodyTy : LamSort}
-  (lctx : Nat → LamSort)
-  (wfArg : LamWF ltv ⟨lctx, LamTerm.bvarLifts arg idx, argTy⟩)
-  (wfBody : LamWF ltv ⟨pushLCtxAt lctx argTy idx, body, bodyTy⟩) :
-  LamWF ltv ⟨lctx, LamTerm.subst idx arg body, bodyTy⟩ :=
-  let wfArg' : LamWF ltv ⟨lctx, LamTerm.bvarLiftsRec arg idx, argTy⟩ := (LamTerm.bvarLifts.equiv arg idx) ▸ wfArg
-  let wfBody' : LamWF ltv ⟨pushLCtxAtRec lctx argTy idx, body, bodyTy⟩ := pushLCtxAt.equivFn lctx argTy idx ▸ wfBody
-  (Eq.symm (LamTerm.subst.equiv ltv idx lctx wfArg' wfBody')) ▸ (LamWF.subst' ltv idx lctx wfArg' wfBody').snd
-
-private def LamWF.subst.equiv (ltv : LamTyVal) (idx : Nat)
-  {arg : LamTerm} {argTy : LamSort}
-  {body : LamTerm} {bodyTy : LamSort}
-  (lctx : Nat → LamSort)
-  (wfArg : LamWF ltv ⟨lctx, LamTerm.bvarLifts arg idx, argTy⟩)
-  (wfBody : LamWF ltv ⟨pushLCtxAt lctx argTy idx, body, bodyTy⟩) :
-  let wfArg' : LamWF ltv ⟨lctx, LamTerm.bvarLiftsRec arg idx, argTy⟩ := (LamTerm.bvarLifts.equiv arg idx) ▸ wfArg
-  let wfBody' : LamWF ltv ⟨pushLCtxAtRec lctx argTy idx, body, bodyTy⟩ := pushLCtxAt.equivFn lctx argTy idx ▸ wfBody
-  HEq (LamWF.subst' ltv idx lctx wfArg' wfBody').snd (LamWF.subst ltv idx lctx wfArg wfBody) :=
-    let wfArg' : LamWF ltv ⟨lctx, LamTerm.bvarLiftsRec arg idx, argTy⟩ := (LamTerm.bvarLifts.equiv arg idx) ▸ wfArg
-    let wfBody' : LamWF ltv ⟨pushLCtxAtRec lctx argTy idx, body, bodyTy⟩ := pushLCtxAt.equivFn lctx argTy idx ▸ wfBody
-    heq_of_eqRec_eq'
-      (motive:=fun x => LamWF ltv ⟨lctx, x, bodyTy⟩)
-      (Eq.symm (LamTerm.subst.equiv ltv idx lctx wfArg' wfBody'))
-      _
-
-def LamWF.subst.correct.{u}
+private def LamWF.subst.correct.{u}
   (lval : LamValuation.{u}) (idx : Nat)
-  {arg : LamTerm} {argTy : LamSort} {body : LamTerm} {bodyTy : LamSort}
-  (lctxTy : Nat → LamSort) (lctxTerm : ∀ n, (lctxTy n).interp lval.ilVal.tyVal)
-  (wfArg : LamWF lval.ilVal.toLamTyVal ⟨lctxTy, LamTerm.bvarLifts arg idx, argTy⟩)
-  (wfBody : LamWF lval.ilVal.toLamTyVal ⟨pushLCtxAt lctxTy argTy idx, body, bodyTy⟩) :
-  let wfSubst := LamWF.subst lval.ilVal.toLamTyVal idx lctxTy wfArg wfBody
-  (LamWF.interp lval (pushLCtxAt lctxTy argTy idx)
-    (pushLCtxAtDep lctxTerm (LamWF.interp lval lctxTy lctxTerm wfArg) idx) wfBody
-  = LamWF.interp lval lctxTy lctxTerm wfSubst) :=
-  let wfArg' : LamWF lval.ilVal.toLamTyVal ⟨lctxTy, LamTerm.bvarLiftsRec arg idx, argTy⟩ := (LamTerm.bvarLifts.equiv arg idx) ▸ wfArg
-  let wfBody' : LamWF lval.ilVal.toLamTyVal ⟨pushLCtxAtRec lctxTy argTy idx, body, bodyTy⟩ := pushLCtxAt.equivFn lctxTy argTy idx ▸ wfBody
-  eq_of_heq (
-    let bArg := LamWF.subst' lval.ilVal.toLamTyVal idx lctxTy wfArg' wfBody'
-    HEq.trans (b := LamWF.interp lval lctxTy lctxTerm bArg.snd) (
-      Eq.symm (LamWF.subst'.correct _ _ _ _ wfArg' wfBody') ▸ (
-        LamWF.interp.heq _
-          (Eq.symm (pushLCtxAt.equivFn _ _ _))
-          (let HEquiv := pushLCtxAtDep.equivFn lctxTerm (LamWF.interp lval lctxTy lctxTerm wfArg) idx
-           HEq.trans (HEq.symm HEquiv) (
-            congr_arg₂_heq _ (pushLCtxAtDepRec lctxTerm) (eq_of_heq (
-              LamWF.interp.heq _ rfl HEq.rfl _ _ (Eq.symm (LamTerm.bvarLifts.equiv _ _))
-            )) HEq.rfl
-          )) _ _ rfl)
-     ) (LamWF.interp.heq _ rfl HEq.rfl _ _ (Eq.symm (LamTerm.subst.equiv _ _ _ _ _)))
-  )
+  {arg : LamTerm} {argTy : LamSort} {body : LamTerm} {bodyTy : LamSort} :
+  (lctxTy : Nat → LamSort) → (lctxTerm : ∀ n, (lctxTy n).interp lval.ilVal.tyVal) →
+  (wfArg : LamWF lval.ilVal.toLamTyVal ⟨lctxTy, LamTerm.bvarLifts idx arg, argTy⟩) →
+  (wfBody : LamWF lval.ilVal.toLamTyVal ⟨pushLCtxAt argTy idx lctxTy, body, bodyTy⟩) →
+  let wfSubst' := LamWF.subst lval.ilVal.toLamTyVal idx lctxTy wfArg wfBody
+  (LamWF.interp lval (pushLCtxAt argTy idx lctxTy)
+    (pushLCtxAtDep (LamWF.interp lval lctxTy lctxTerm wfArg) idx lctxTerm) wfBody
+  = LamWF.interp lval lctxTy lctxTerm wfSubst')
+| lctxTy, lctxTerm, wfArg, .ofAtom n => rfl
+| lctxTy, lctxTerm, wfArg, .ofBase b => rfl
+| lctxTy, lctxTerm, wfArg, .ofBVar n => by
+  dsimp [LamWF.interp, LamWF.subst, LamTerm.subst]
+  dsimp [pushLCtxAt, pushLCtxAtDep, restoreAt, restoreAtDep, pushLCtx]
+  match Nat.ble idx n with
+  | true =>
+    dsimp;
+    match (n - idx) with
+    | 0 => rfl
+    | _ + 1 => rfl
+  | false => rfl
+| lctxTy, lctxTerm, wfArg, .ofLam (argTy:=argTy') bodyTy' (body:=body') H =>
+  funext (fun x => by
+    let wfArg' := LamWF.ofBVarLiftIdx (s:=argTy') (lctx:=lctxTy) 0 _ wfArg
+    rw [pushLCtxAt.zero] at wfArg'
+    dsimp [LamTerm.bvarLifts] at wfArg'
+    rw [← LamTerm.bvarLiftsIdx.succ_r] at wfArg'
+    rw [pushLCtx_pushLCtxAt] at H
+    let IH := LamWF.subst.correct lval (.succ idx) (pushLCtx argTy' lctxTy) (pushLCtxDep x lctxTerm) wfArg' H
+    apply Eq.trans _ (Eq.trans IH _)
+    case _ =>
+      dsimp [interp]; apply eq_of_heq; apply interp.heq <;> try rfl
+      case h.HLCtxTyEq => apply pushLCtx_pushLCtxAt
+      case h.HLCtxTermEq =>
+        apply HEq.trans (pushLCtxDep_pushLCtxAtDep _ _ _ _)
+        apply heq_of_eq
+        apply congr_arg (f := fun x => pushLCtxAtDep x _ _)
+        rw [LamWF.ofBVarLiftIdx.correct (idx:=0) lval _ lctxTerm x _ wfArg]
+        apply eq_of_heq; apply interp.heq
+        case h.h.HLCtxTyEq => rw [pushLCtxAt.zero]
+        case h.h.HLCtxTermEq => apply pushLCtxAtDep.zero
+        case h.h.HTeq => rw [← LamTerm.bvarLiftsIdx.succ_r]
+    case _ =>
+      dsimp [interp]; apply eq_of_heq; apply interp.heq <;> rfl)
+| lctxTy, lctxTerm, wfArg, .ofApp argTy' HFn HArg =>
+  let IHFn := LamWF.subst.correct lval idx lctxTy lctxTerm wfArg HFn
+  let IHArg := LamWF.subst.correct lval idx lctxTy lctxTerm wfArg HArg
+  by dsimp [LamWF.interp]; dsimp at IHFn; dsimp at IHArg; simp [IHFn, IHArg]
+
 
 -- Note: `LamTerm.subst`, `LamWF.subst` and `LamWF.subst_correct` is the main API
 --   of syntactic operations on `λ` terms
@@ -301,12 +118,14 @@ def LamWF.headBetaAux (ltv : LamTyVal)
   | .atom _  => .ofApp _ wfFn wfArg
   | .base _  => .ofApp _ wfFn wfArg
   | .bvar _  => .ofApp _ wfFn wfArg
-  | .lam s body =>
+  | .lam _ body =>
     match argTy, wfFn with
     | _, .ofLam (argTy:=argTy') (body:=body') bodyTy' wfBody =>
-      LamWF.subst ltv 0 lctx
-        (by rw [LamTerm.bvarLifts.zero]; exact wfArg)
-        (by rw [← pushLCtxAt.equivFn]; exact wfBody)
+      LamWF.subst ltv 0 lctx (argTy:=argTy')
+        (by dsimp [LamTerm.bvarLifts];
+            rw [LamTerm.bvarLiftsIdx.zero 0 arg];
+            exact wfArg)
+        (by rw [pushLCtxAt.zero]; exact wfBody)
   | .app _ _ => .ofApp _ wfFn wfArg
 
 def LamWF.headBetaAux.correct.{u} (lval : LamValuation.{u})
@@ -326,21 +145,20 @@ def LamWF.headBetaAux.correct.{u} (lval : LamValuation.{u})
     | _, .ofLam (argTy:=_) (body:=_) _ wfBody => by
       dsimp [headBetaAux, LamWF.interp]
       let b := LamWF.interp lval
-        (pushLCtxAt lctxTy s 0)
-        (pushLCtxAtDep lctxTerm (LamWF.interp lval lctxTy lctxTerm wfArg) 0)
-        (by rw [← pushLCtxAt.equivFn]; exact wfBody)
+        (pushLCtxAt s 0 lctxTy)
+        (pushLCtxAtDep (LamWF.interp lval lctxTy lctxTerm wfArg) 0 lctxTerm)
+        (by rw [pushLCtxAt.zero]; exact wfBody)
       apply Eq.trans (b:=b)
       case h₁ =>
         apply eq_of_heq; apply LamWF.interp.heq <;> try rfl
-        rw [← pushLCtxAt.equivFn]; rfl
-        exact (pushLCtxAtDep.equivFn lctxTerm _ 0)
+        rw [pushLCtxAt.zero]; apply HEq.symm; apply pushLCtxAtDep.zero
       case h₂ =>
         dsimp
         rw [← LamWF.subst.correct]
         apply eq_of_heq; apply LamWF.interp.heq <;> try rfl
-        apply heq_of_eq; apply congr_fun; apply congr_arg;
+        apply heq_of_eq; apply congr_arg (f := fun x => pushLCtxAtDep x 0 lctxTerm);
         apply eq_of_heq; apply LamWF.interp.heq <;> try rfl
-        rw [LamTerm.bvarLifts.zero]
+        dsimp [LamTerm.bvarLifts]; rw [LamTerm.bvarLiftsIdx.zero 0 arg]
   | .app _ _ => rfl
 
 def LamTerm.headBeta : LamTerm → LamTerm
